progress: some cases

Capless/Soundness/Progress.lean
@@ -2,19 +2,36 @@ import Capless.Reduction
 namespace Capless
 
 inductive Progress : State n m k -> Prop where
-| mk :
+| step :
   Reduce state state' ->
   Progress state
+| halt_value {t : Term n m k} :
+  t.IsValue ->
+  Progress ⟨σ, Cont.none, t⟩
+| halt_var :
+  Progress ⟨σ, Cont.none, Term.var x⟩
 
 theorem progress
   (ht : TypedState state E) :
   Progress state := by
   cases ht
   case mk hs ht hc =>
-    cases ht
-    case var => sorry
-    case pack => sorry
-    case sub => sorry
+    induction ht
+    case var =>
+      cases hc
+      case none => apply Progress.halt_var
+      case cons =>
+        apply Progress.step
+        apply Reduce.rename
+    case pack =>
+      cases hc
+      case none => apply Progress.halt_value; constructor
+      case conse =>
+        apply Progress.step
+        apply Reduce.lift_ex
+    case sub hsub ih _ _ =>
+      apply ih <;> try trivial
+      sorry
     case abs => sorry
     case tabs => sorry
     case cabs => sorry
